final changes

avl-py/module_.py
@@ -1,0 +1,401 @@
+import sys
+from typing import Callable, Any, TypeVar, NamedTuple
+from math import floor
+from itertools import count
+
+import module_ as module_
+import _dafny as _dafny
+import System_ as System_
+
+# Module: module_
+
+class default__:
+    def  __init__(self):
+        pass
+
+    @staticmethod
+    def TestAVLNode():
+        d_0_root_: AVLNode
+        nw0_ = AVLNode()
+        nw0_.ctor__(10)
+        d_0_root_ = nw0_
+        d_1_leftChild_: AVLNode
+        nw1_ = AVLNode()
+        nw1_.ctor__(5)
+        d_1_leftChild_ = nw1_
+        d_2_rightChild_: AVLNode
+        nw2_ = AVLNode()
+        nw2_.ctor__(15)
+        d_2_rightChild_ = nw2_
+        (d_0_root_).left = d_1_leftChild_
+        (d_0_root_).right = d_2_rightChild_
+        (d_0_root_).UpdateHeight()
+
+    @staticmethod
+    def TestBalanceFactors():
+        d_0_root_: AVLNode
+        nw0_ = AVLNode()
+        nw0_.ctor__(20)
+        d_0_root_ = nw0_
+        d_1_left_: AVLNode
+        nw1_ = AVLNode()
+        nw1_.ctor__(10)
+        d_1_left_ = nw1_
+        d_2_leftLeft_: AVLNode
+        nw2_ = AVLNode()
+        nw2_.ctor__(5)
+        d_2_leftLeft_ = nw2_
+        (d_1_left_).left = d_2_leftLeft_
+        (d_1_left_).UpdateHeight()
+        (d_0_root_).left = d_1_left_
+        (d_0_root_).UpdateHeight()
+        d_3_right_: AVLNode
+        nw3_ = AVLNode()
+        nw3_.ctor__(30)
+        d_3_right_ = nw3_
+        d_4_rightRight_: AVLNode
+        nw4_ = AVLNode()
+        nw4_.ctor__(35)
+        d_4_rightRight_ = nw4_
+        (d_3_right_).right = d_4_rightRight_
+        (d_3_right_).UpdateHeight()
+        (d_0_root_).right = d_3_right_
+        (d_0_root_).UpdateHeight()
+
+    @staticmethod
+    def TestSingleNode():
+        d_0_node_: AVLNode
+        nw0_ = AVLNode()
+        nw0_.ctor__(42)
+        d_0_node_ = nw0_
+
+    @staticmethod
+    def Main(noArgsParameter__):
+        default__.TestAVLNode()
+        default__.TestBalanceFactors()
+        default__.TestSingleNode()
+        d_0_cmp_: IntComparator
+        nw0_ = IntComparator()
+        nw0_.ctor__()
+        d_0_cmp_ = nw0_
+        d_1_tree_: AVLTree
+        nw1_ = AVLTree()
+        nw1_.ctor__(d_0_cmp_)
+        d_1_tree_ = nw1_
+        d_2_b_: bool
+        out0_: bool
+        out0_ = (d_1_tree_).IsEmpty()
+        d_2_b_ = out0_
+        nw2_ = AVLNode()
+        nw2_.ctor__(10)
+        (d_1_tree_).root = nw2_
+        obj0_ = d_1_tree_.root
+        nw3_ = AVLNode()
+        nw3_.ctor__(5)
+        obj0_.left = nw3_
+        obj1_ = d_1_tree_.root
+        nw4_ = AVLNode()
+        nw4_.ctor__(15)
+        obj1_.right = nw4_
+        (d_1_tree_.root.left).UpdateHeight()
+        (d_1_tree_.root.right).UpdateHeight()
+        (d_1_tree_.root).UpdateHeight()
+
+
+class AVLNode:
+    def  __init__(self):
+        self.data: TypeVar('T') = None
+        self.left: AVLNode = None
+        self.right: AVLNode = None
+        self.height: int = int(0)
+        pass
+
+    def __dafnystr__(self) -> str:
+        return "_module.AVLNode"
+    def ctor__(self, value):
+        (self).data = value
+        (self).left = None
+        (self).right = None
+        (self).height = 1
+
+    def Height(self):
+        return self.height
+
+    def LeftHeight(self):
+        if (self.left) == (None):
+            return 0
+        elif True:
+            return self.left.height
+
+    def RightHeight(self):
+        if (self.right) == (None):
+            return 0
+        elif True:
+            return self.right.height
+
+    def BalanceFactor(self):
+        return ((self).RightHeight()) - ((self).LeftHeight())
+
+    def IsBalanced(self):
+        d_0_bf_ = (self).BalanceFactor()
+        return ((-1) <= (d_0_bf_)) and ((d_0_bf_) <= (1))
+
+    def HeightValid(self):
+        return (self.height) == ((1) + (((self).LeftHeight() if ((self).LeftHeight()) > ((self).RightHeight()) else (self).RightHeight())))
+
+    def ValidAVLNode(self):
+        return ((((self).HeightValid()) and ((self).IsBalanced())) and (((self.left) == (None)) or ((self.left).ValidAVLNode()))) and (((self.right) == (None)) or ((self.right).ValidAVLNode()))
+
+    def UpdateHeight(self):
+        d_0_leftH_: int
+        d_0_leftH_ = (self).LeftHeight()
+        d_1_rightH_: int
+        d_1_rightH_ = (self).RightHeight()
+        d_2_maxH_: int
+        if (d_0_leftH_) > (d_1_rightH_):
+            d_2_maxH_ = d_0_leftH_
+        elif True:
+            d_2_maxH_ = d_1_rightH_
+        (self).height = (1) + (d_2_maxH_)
+
+    def LeftRotate(self):
+        newRoot: AVLNode = None
+        d_0_pivot_: AVLNode
+        d_0_pivot_ = self.right
+        d_1_temp_: AVLNode
+        d_1_temp_ = d_0_pivot_.left
+        (d_0_pivot_).left = self
+        (self).right = d_1_temp_
+        (self).UpdateHeight()
+        (d_0_pivot_).UpdateHeight()
+        newRoot = d_0_pivot_
+        return newRoot
+
+    def RightRotate(self):
+        newRoot: AVLNode = None
+        d_0_pivot_: AVLNode
+        d_0_pivot_ = self.left
+        d_1_temp_: AVLNode
+        d_1_temp_ = d_0_pivot_.right
+        (d_0_pivot_).right = self
+        (self).left = d_1_temp_
+        (self).UpdateHeight()
+        (d_0_pivot_).UpdateHeight()
+        newRoot = d_0_pivot_
+        return newRoot
+
+    def LeftRightRotate(self):
+        newRoot: AVLNode = None
+        d_0_a_: AVLNode
+        d_0_a_ = self
+        d_1_b_: AVLNode
+        d_1_b_ = self.left
+        d_2_c_: AVLNode
+        d_2_c_ = self.left.right
+        d_3_t1_: AVLNode
+        d_3_t1_ = d_2_c_.left
+        d_4_t2_: AVLNode
+        d_4_t2_ = d_2_c_.right
+        (d_2_c_).left = d_1_b_
+        (d_2_c_).right = d_0_a_
+        (d_1_b_).right = d_3_t1_
+        (d_0_a_).left = d_4_t2_
+        (d_1_b_).UpdateHeight()
+        (d_0_a_).UpdateHeight()
+        (d_2_c_).UpdateHeight()
+        newRoot = d_2_c_
+        return newRoot
+
+    def RightLeftRotate(self):
+        newRoot: AVLNode = None
+        d_0_a_: AVLNode
+        d_0_a_ = self
+        d_1_b_: AVLNode
+        d_1_b_ = self.right
+        d_2_c_: AVLNode
+        d_2_c_ = self.right.left
+        d_3_t1_: AVLNode
+        d_3_t1_ = d_2_c_.left
+        d_4_t2_: AVLNode
+        d_4_t2_ = d_2_c_.right
+        (d_2_c_).left = d_0_a_
+        (d_2_c_).right = d_1_b_
+        (d_0_a_).right = d_3_t1_
+        (d_1_b_).left = d_4_t2_
+        (d_0_a_).UpdateHeight()
+        (d_1_b_).UpdateHeight()
+        (d_2_c_).UpdateHeight()
+        newRoot = d_2_c_
+        return newRoot
+
+    def IsLeaf(self):
+        return ((self.left) == (None)) and ((self.right) == (None))
+
+    def HasOneChild(self):
+        return (((self.left) == (None)) and ((self.right) != (None))) or (((self.left) != (None)) and ((self.right) == (None)))
+
+    def HasTwoChildren(self):
+        return ((self.left) != (None)) and ((self.right) != (None))
+
+    def Insert(self, value, cmp):
+        newRoot: AVLNode = None
+        d_0_isEqual_: bool
+        out0_: bool
+        out0_ = (cmp).Equal(self.data, value)
+        d_0_isEqual_ = out0_
+        if d_0_isEqual_:
+            newRoot = self
+            return newRoot
+        d_1_isLess_: bool
+        out1_: bool
+        out1_ = (cmp).Less(value, self.data)
+        d_1_isLess_ = out1_
+        if d_1_isLess_:
+            if (self.left) == (None):
+                nw0_ = AVLNode()
+                nw0_.ctor__(value)
+                (self).left = nw0_
+        elif True:
+            if (self.right) == (None):
+                nw1_ = AVLNode()
+                nw1_.ctor__(value)
+                (self).right = nw1_
+        (self).UpdateHeight()
+        newRoot = self
+        return newRoot
+
+    def FindMinNode(self):
+        minNode: AVLNode = None
+        d_0_current_: AVLNode
+        d_0_current_ = self
+        while (d_0_current_.left) != (None):
+            d_0_current_ = d_0_current_.left
+        minNode = d_0_current_
+        return minNode
+
+    def Rebalance(self):
+        newRoot: AVLNode = None
+        newRoot = self
+        return newRoot
+
+    def Delete(self, value, cmp):
+        newRoot: AVLNode = None
+        d_0_isEqual_: bool
+        out0_: bool
+        out0_ = (cmp).Equal(self.data, value)
+        d_0_isEqual_ = out0_
+        if d_0_isEqual_:
+            if (self).IsLeaf():
+                newRoot = None
+                return newRoot
+            elif (self).HasOneChild():
+                if (self.left) == (None):
+                    newRoot = self.right
+                elif True:
+                    newRoot = self.left
+                return newRoot
+            elif True:
+                pass
+        elif True:
+            newRoot = self
+        return newRoot
+
+
+class Comparator:
+    pass
+    def Less(self, x, y):
+        pass
+
+    def Equal(self, x, y):
+        pass
+
+
+class IntComparator(Comparator):
+    def  __init__(self):
+        pass
+
+    def __dafnystr__(self) -> str:
+        return "_module.IntComparator"
+    def ctor__(self):
+        pass
+        pass
+
+    def Less(self, x, y):
+        b: bool = False
+        b = (x) < (y)
+        return b
+
+    def Equal(self, x, y):
+        b: bool = False
+        b = (x) == (y)
+        return b
+
+
+class AVLTree:
+    def  __init__(self):
+        self.root: AVLNode = None
+        self.cmp: Comparator = None
+        pass
+
+    def __dafnystr__(self) -> str:
+        return "_module.AVLTree"
+    def ctor__(self, c):
+        (self).root = None
+        (self).cmp = c
+
+    def Valid(self):
+        return ((self.root) == (None)) or ((self.root).ValidAVLNode())
+
+    def IsEmpty(self):
+        empty: bool = False
+        empty = (self.root) == (None)
+        return empty
+
+    def GetHeight(self):
+        h: int = int(0)
+        if (self.root) == (None):
+            h = 0
+        elif True:
+            h = self.root.height
+        return h
+
+    def Search(self, value):
+        found: bool = False
+        d_0_current_: AVLNode
+        d_0_current_ = self.root
+        while (d_0_current_) != (None):
+            d_1_isEqual_: bool
+            out0_: bool
+            out0_ = (self.cmp).Equal(d_0_current_.data, value)
+            d_1_isEqual_ = out0_
+            if d_1_isEqual_:
+                found = True
+                return found
+            d_2_isLess_: bool
+            out1_: bool
+            out1_ = (self.cmp).Less(value, d_0_current_.data)
+            d_2_isLess_ = out1_
+            if d_2_isLess_:
+                d_0_current_ = d_0_current_.left
+            elif True:
+                d_0_current_ = d_0_current_.right
+        found = False
+        return found
+
+    def Insert(self, value):
+        if (self.root) == (None):
+            nw0_ = AVLNode()
+            nw0_.ctor__(value)
+            (self).root = nw0_
+        elif True:
+            d_0___v0_: AVLNode
+            out0_: AVLNode
+            out0_ = (self.root).Insert(value, self.cmp)
+            d_0___v0_ = out0_
+
+    def Delete(self, value):
+        if (self.root) != (None):
+            out0_: AVLNode
+            out0_ = (self.root).Delete(value, self.cmp)
+            (self).root = out0_
+
